work in progress after discussion with Tim

SyBlocToObc/Correctness.v
@@ -12,6 +12,9 @@ Require Import Velus.SyBloc.SBSemantics.
 Require Import Velus.Obc.ObcSyntax.
 Require Import Velus.Obc.ObcSemantics.
 
+Require Import Velus.NLustre.NLSyntax.
+Require Export Velus.NLustre.IsFree.
+
 Require Import Velus.SyBlocToObc.Translation.
 
 Require Import List.
@@ -28,374 +31,744 @@ Module Type CORRECTNESS
        (Import OpAux   : OPERATORS_AUX       Op)
        (Import Clks    : CLOCKS          Ids)
        (Import ExprSyn : NLEXPRSYNTAX        Op)
+       (SynNL          : NLSYNTAX        Ids Op       Clks ExprSyn)
        (Import SynSB   : SBSYNTAX        Ids Op       Clks ExprSyn)
        (Import Str     : STREAM              Op OpAux)
        (Import ExprSem : NLEXPRSEMANTICS Ids Op OpAux Clks ExprSyn              Str)
        (Import SemSB   : SBSEMANTICS     Ids Op OpAux Clks ExprSyn SynSB        Str ExprSem)
        (Import SynObc  : OBCSYNTAX       Ids Op OpAux)
        (Import SemObc  : OBCSEMANTICS    Ids Op OpAux                    SynObc)
-       (Import Trans   : TRANSLATION     Ids Op OpAux Clks ExprSyn SynSB SynObc).
+       (Import Trans   : TRANSLATION     Ids Op OpAux Clks ExprSyn SynSB SynObc)
+       (Import IsF     : ISFREE          Ids Op       Clks ExprSyn SynNL).
 
-  Definition compat_env (R: env) (mems: PS.t) (me: menv) (ve: venv) :=
+  Section MemoryCorres.
+
+    Variable P: SynSB.program.
+
+    Inductive Memory_Corres: ident -> state -> menv -> Prop :=
+      MemC:
+        forall b S me bl P',
+          find_block b P = Some (bl, P') ->
+          Forall (Memory_Corres_eq S me) bl.(b_eqs) ->
+          Memory_Corres b S me
+
+    with Memory_Corres_eq: state -> menv -> equation -> Prop :=
+         | MemC_EqDef:
+             forall S me x ck e,
+               Memory_Corres_eq S me (EqDef x ck e)
+         | MemC_EqNext:
+             forall S me x ck e,
+               (forall v, find_val x S = Some v ->
+                     find_val x me = Some v) ->
+               Memory_Corres_eq S me (EqNext x ck e)
+         | MemC_EqReset:
+             forall S me s ck b,
+               (forall Ss, sub_inst s S Ss ->
+                    exists me', sub_inst s me me') ->
+               Memory_Corres_eq S me (EqReset s ck b)
+         | MemC_EqCall:
+           forall S me s xs ck rst b es,
+             (forall Ss, sub_inst s S Ss ->
+                    exists me', sub_inst s me me'
+                           /\ Memory_Corres b Ss me') ->
+             Memory_Corres_eq S me (EqCall s xs ck rst b es).
+
+    Definition Memory_Corres_eqs (S: state) (me: menv) (eqs: list equation) :=
+      Forall (Memory_Corres_eq S me) eqs.
+
+    Section MemoryCorresMult.
+
+      Variable P_block: ident -> state -> menv -> Prop.
+      Variable P_equation: state -> menv -> equation -> Prop.
+
+      Hypothesis EqDef_case:
+        forall S me x ck e,
+          P_equation S me (EqDef x ck e).
+
+      Hypothesis EqNext_case:
+        forall S me x ck e,
+          (forall v, find_val x S = Some v ->
+                find_val x me = Some v) ->
+          P_equation S me (EqNext x ck e).
+
+      Hypothesis EqReset_case:
+        forall S me s ck b,
+          (forall Ss, sub_inst s S Ss ->
+                 exists me', sub_inst s me me') ->
+          P_equation S me (EqReset s ck b).
+
+      Hypothesis EqCall_case:
+        forall S me s xs ck rst b es,
+          (forall Ss, sub_inst s S Ss ->
+                 exists me', sub_inst s me me'
+                        /\ Memory_Corres b Ss me'
+                        /\ P_block b Ss me') ->
+          P_equation S me (EqCall s xs ck rst b es).
+
+      Hypothesis MemC_case:
+        forall b S me bl P',
+          find_block b P = Some (bl, P') ->
+          Forall (Memory_Corres_eq S me) bl.(b_eqs) ->
+          Forall (P_equation S me) bl.(b_eqs) ->
+          P_block b S me.
+
+      Fixpoint Memory_Corres_mult
+               (b: ident) (S: state) (me: menv)
+               (Hmc: Memory_Corres b S me):
+        P_block b S me
+      with Memory_Corres_eq_mult
+             (S: state) (me: menv) (eq: equation)
+             (Hmceq: Memory_Corres_eq S me eq):
+             P_equation S me eq.
+      Proof.
+        - destruct Hmc. eauto.
+          eapply MemC_case; eauto.
+          match goal with H: Forall _ _ |- _ => induction H; auto end.
+        - destruct Hmceq as [| | |???????? Spec]; eauto.
+          apply EqCall_case.
+          intros ** Sub; apply Spec in Sub as (?&?&?); eauto.
+      Qed.
+
+    End MemoryCorresMult.
+
+  End MemoryCorres.
+
+  Lemma Memory_Corres_eqs_add_val:
+    forall P S me x v eqs,
+      find_val x S = Some v ->
+      Memory_Corres_eqs P S me eqs ->
+      Memory_Corres_eqs P S (add_val x v me) eqs.
+  Proof.
+    unfold Memory_Corres_eqs.
+    induction eqs as [|eq]; auto.
+    intros Find; inversion_clear 1 as [|?? Corres].
+    constructor; auto.
+    destruct eq; constructor; inv Corres; eauto.
+    intros ** Find'.
+    destruct (ident_eq_dec i x).
+    - subst; rewrite find_val_gss; congruence.
+    - rewrite find_val_gso; auto.
+  Qed.
+
+  Definition equiv_env (in_domain: ident -> Prop) (R: env) (mems: PS.t) (me: menv) (ve: venv) : Prop :=
     forall x c,
-      Env.find x R = Some (present c) ->
+      in_domain x ->
+      sem_var_instant R x (present c) ->
       if PS.mem x mems
       then find_val x me = Some c
       else Env.find x ve = Some c.
 
-  Section BuildMemWith.
-
-    Context {A B V: Type}.
-    Variable f: A -> V.
-    Variable g: B -> memory V.
-
-    Definition build_mem_with (xs: list (ident * A)) (ys: list (ident * B)) (m: memory V): memory V :=
-      fold_left (fun m x => add_inst (fst x) (g (snd x)) m) ys
-                (fold_left (fun m y => add_val (fst y) (f (snd y)) m) xs m).
-
-    Definition build_mem_with_spec (xs: list (ident * A)) (ys: list (ident * B)) (m: memory V): memory V :=
-      let (xs, vs) := split xs in
-      let (ys, ws) := split ys in
-      Mem (Env.adds xs (map f vs) (values m)) (Env.adds ys (map g ws) (instances m)).
-
-    Lemma build_mem_with_spec_values:
-      forall xs ys m,
-        values (build_mem_with_spec xs ys m) =
-        let (xs, vs) := split xs in
-        Env.adds xs (map f vs) (values m).
-    Proof.
-      intros; unfold build_mem_with_spec; destruct (split xs), (split ys); auto.
-    Qed.
-
-    Lemma build_mem_with_spec_instances:
-      forall xs ys m,
-        instances (build_mem_with_spec xs ys m) =
-        let (ys, ws) := split ys in
-        Env.adds ys (map g ws) (instances m).
-    Proof.
-      intros; unfold build_mem_with_spec; destruct (split xs), (split ys); auto.
-    Qed.
-
-    Lemma build_mem_with_equal:
-      forall ys xs m,
-        NoDupMembers ys ->
-        NoDupMembers xs ->
-        build_mem_with xs ys m ≋ build_mem_with_spec xs ys m.
-    Proof.
-      unfold build_mem_with, build_mem_with_spec.
-      induction ys as [|(y, b)]; intros ** NoDup_ys NoDup_xs; simpl.
-      - rewrite Env.adds_nil_nil.
-        revert m.
-        induction xs as [|(x, a)]; intro; simpl.
-        + now rewrite Env.adds_nil_nil.
-        + inversion_clear NoDup_xs as [|??? Notin].
-          rewrite IHxs; auto.
-          destruct (split xs) eqn: E; simpl.
-          rewrite Env.adds_cons_cons; try reflexivity.
-          replace l with (fst (split xs)); [|now rewrite E].
-          intro Hin; apply Notin.
-          apply in_split_l' in Hin as (?&?).
-          eapply In_InMembers; eauto.
-      - destruct (split xs) eqn: Exs, (split ys) as (l') eqn: Eys; simpl in *.
-        inversion_clear NoDup_ys as [|??? Notin].
-        rewrite Env.adds_cons_cons.
-        + set (m' := add_inst y (g b) m).
-          change (Env.add y (g b) (instances m)) with (instances m');
-            change (values m) with (values m').
-          apply (IHys _ m') in NoDup_xs; auto.
-          rewrite Exs in NoDup_xs.
-          rewrite <-NoDup_xs.
-          subst m'; clear; revert m.
-          induction xs as [|(x', a')]; intros; simpl; try reflexivity.
-          rewrite IHxs.
-          now rewrite add_inst_val_comm.
-        + replace l' with (fst (split ys)); [|now rewrite Eys].
-          intro Hin; apply Notin.
-          apply in_split_l' in Hin as (?&?).
-          eapply In_InMembers; eauto.
-    Qed.
-
-  End BuildMemWith.
-
-  Add Parametric Morphism A B V f xs ys m: (fun g => @build_mem_with_spec A B V f g xs ys m)
-      with signature (fun g g' => forall x, g x ≋ g' x) ==> equal_memory
-        as build_mem_with_spec_rec_equal_memory.
+  Lemma equiv_env_map:
+    forall (in_dom1 in_dom2: ident -> Prop) R mems me ve,
+      (forall x, in_dom2 x -> in_dom1 x) ->
+      equiv_env in_dom1 R mems me ve ->
+      equiv_env in_dom2 R mems me ve.
   Proof.
-    intros g g' E.
-    unfold build_mem_with_spec.
-    induction ys as [|(y, b)]; simpl; try reflexivity.
-    destruct (split ys); simpl.
-    unfold Env.adds. simpl.
-    destruct (split xs); simpl.
-    constructor; try reflexivity.
-    simpl.
-    inversion_clear IHys as [??? Insts].
-    unfold Env.adds in Insts; simpl in Insts.
-    now rewrite E, Insts.
+    unfold equiv_env; intros ** Eq ????; apply Eq; auto.
   Qed.
 
-  Fixpoint reset_state_spec (P: SynSB.program) (b: ident) : state :=
-    match P with
-    | [] => empty_memory _
-    | bl :: P =>
-      if ident_eqb (b_name bl) b
-      then build_mem_with_spec sem_const (reset_state_spec P) (b_lasts bl) (b_blocks bl) (empty_memory _)
-      else reset_state_spec P b
+  Ltac weaken_equiv_env_with tac :=
+    match goal with
+      H: equiv_env ?in_dom1 ?R ?mems ?me ?ve
+      |- equiv_env ?in_dom2 ?R ?mems ?me ?ve =>
+      eapply equiv_env_map; [|exact H]; tac
     end.
 
-  Fixpoint reset_state (P: SynSB.program) (b: ident) : state :=
-    match P with
-    | [] => empty_memory _
-    | bl :: P =>
-      if ident_eqb (b_name bl) b
-      then build_mem_with sem_const (reset_state P) (b_lasts bl) (b_blocks bl) (empty_memory _)
-      else reset_state P b
-    end.
+  Tactic Notation "weaken_equiv_env" "with" tactic(tac) :=
+    weaken_equiv_env_with tac.
 
-  Lemma reset_state_equal:
-    forall P b,
-      reset_state P b ≋ reset_state_spec P b.
+  Tactic Notation "weaken_equiv_env" :=
+    weaken_equiv_env with constructor (now auto).
+
+  Hint Extern 4 (equiv_env _ _ _ _ _) => weaken_equiv_env.
+
+  Inductive Is_defined_in_eq: ident -> equation -> Prop :=
+  | DefEqDef:
+      forall x ck e,
+        Is_defined_in_eq x (EqDef x ck e)
+  | DefEqNext:
+      forall x ck e,
+        Is_defined_in_eq x (EqNext x ck e)
+  | DefEqCall:
+      forall x s xs ck rst b es,
+        In x xs ->
+        Is_defined_in_eq x (EqCall s xs ck rst b es).
+
+  Definition Is_defined_in_eqs (x: ident) (eqs: list equation) : Prop :=
+    Exists (Is_defined_in_eq x) eqs.
+
+  Inductive Is_variable_in_eq: ident -> equation -> Prop :=
+  | VarEqDef:
+      forall x ck e,
+        Is_variable_in_eq x (EqDef x ck e)
+  | VarEqCall:
+      forall x s xs ck rst b es,
+        In x xs ->
+        Is_variable_in_eq x (EqCall s xs ck rst b es).
+
+  Definition Is_variable_in_eqs (x: ident) (eqs: list equation) : Prop :=
+    Exists (Is_variable_in_eq x) eqs.
+
+  Inductive Is_state_in_eq: ident -> equation -> nat -> Prop :=
+  | StateEqReset:
+      forall s ck b,
+        Is_state_in_eq s (EqReset s ck b) 0
+  | StateEqCall:
+      forall s xs ck rst b es,
+        Is_state_in_eq s (EqCall s xs ck rst b es) 1.
+
+  Inductive Is_free_in_eq: ident -> equation -> Prop :=
+  | FreeEqDef:
+      forall x ck e y,
+        Is_free_in_caexp y ck e ->
+        Is_free_in_eq y (EqDef x ck e)
+  | FreeEqNext:
+      forall x ck e y,
+        Is_free_in_laexp y ck e ->
+        Is_free_in_eq y (EqNext x ck e)
+  | FreeEqReset:
+      forall s ck b x,
+        Is_free_in_clock x ck ->
+        Is_free_in_eq x (EqReset s ck b)
+  | FreeEqCall:
+      forall s x ck rst b es y,
+        Is_free_in_laexps y ck es ->
+        Is_free_in_eq y (EqCall s x ck rst b es).
+
+  Inductive Is_well_sch (inputs: list ident) (mems: PS.t): list equation -> Prop :=
+  | WSchNil:
+      Is_well_sch inputs mems []
+  | WSchEq:
+      forall eq eqs,
+        Is_well_sch inputs mems eqs ->
+        (forall x,
+            Is_free_in_eq x eq ->
+            if PS.mem x mems
+            then ~ Is_defined_in_eqs x eqs
+            else Is_variable_in_eqs x eqs \/ In x inputs) ->
+        (forall x, Is_defined_in_eq x eq -> ~ Is_defined_in_eqs x eqs) ->
+        (forall s k,
+            Is_state_in_eq s eq k ->
+            Forall (fun eq => forall k', Is_state_in_eq s eq k' -> k' < k) eqs) ->
+        Is_well_sch inputs mems (eq :: eqs).
+
+  (* Section BuildMemWith. *)
+
+  (*   Context {A B V: Type}. *)
+  (*   Variable f: A -> V. *)
+  (*   Variable g: ident * B -> memory V. *)
+
+  (*   Definition build_mem_with (xs: list (ident * A)) (ys: list (ident * B)) (m: memory V): memory V := *)
+  (*     fold_left (fun m x => add_inst (fst x) (g x) m) ys *)
+  (*               (fold_left (fun m y => add_val (fst y) (f (snd y)) m) xs m). *)
+
+  (*   Definition build_mem_with_spec (xs: list (ident * A)) (ys: list (ident * B)) (m: memory V): memory V := *)
+  (*     let (xs, vs) := split xs in *)
+  (*     let (ys', ws) := split ys in *)
+  (*     Mem (Env.adds xs (map f vs) (values m)) (Env.adds ys' (map g ys) (instances m)). *)
+
+  (*   Lemma build_mem_with_spec_values: *)
+  (*     forall xs ys m, *)
+  (*       values (build_mem_with_spec xs ys m) = *)
+  (*       let (xs, vs) := split xs in *)
+  (*       Env.adds xs (map f vs) (values m). *)
+  (*   Proof. *)
+  (*     intros; unfold build_mem_with_spec; destruct (split xs), (split ys); auto. *)
+  (*   Qed. *)
+
+  (*   Lemma build_mem_with_spec_instances: *)
+  (*     forall xs ys m, *)
+  (*       instances (build_mem_with_spec xs ys m) = *)
+  (*       let (ys', ws) := split ys in *)
+  (*       Env.adds ys' (map g ys) (instances m). *)
+  (*   Proof. *)
+  (*     intros; unfold build_mem_with_spec; destruct (split xs), (split ys); auto. *)
+  (*   Qed. *)
+
+  (*   Lemma build_mem_with_equal: *)
+  (*     forall ys xs m, *)
+  (*       NoDupMembers ys -> *)
+  (*       NoDupMembers xs -> *)
+  (*       build_mem_with xs ys m ≋ build_mem_with_spec xs ys m. *)
+  (*   Proof. *)
+  (*     unfold build_mem_with, build_mem_with_spec. *)
+  (*     induction ys as [|(y, b)]; intros ** NoDup_ys NoDup_xs; simpl. *)
+  (*     - rewrite Env.adds_nil_nil. *)
+  (*       revert m. *)
+  (*       induction xs as [|(x, a)]; intro; simpl. *)
+  (*       + now rewrite Env.adds_nil_nil. *)
+  (*       + inversion_clear NoDup_xs as [|??? Notin]. *)
+  (*         rewrite IHxs; auto. *)
+  (*         destruct (split xs) eqn: E; simpl. *)
+  (*         rewrite Env.adds_cons_cons; try reflexivity. *)
+  (*         replace l with (fst (split xs)); [|now rewrite E]. *)
+  (*         intro Hin; apply Notin. *)
+  (*         apply in_split_l' in Hin as (?&?). *)
+  (*         eapply In_InMembers; eauto. *)
+  (*     - destruct (split xs) eqn: Exs, (split ys) as (l') eqn: Eys; simpl in *. *)
+  (*       inversion_clear NoDup_ys as [|??? Notin]. *)
+  (*       rewrite Env.adds_cons_cons. *)
+  (*       + set (m' := add_inst y (g (y, b)) m). *)
+  (*         change (Env.add y (g (y, b)) (instances m)) with (instances m'); *)
+  (*           change (values m) with (values m'). *)
+  (*         apply (IHys _ m') in NoDup_xs; auto. *)
+  (*         rewrite Exs in NoDup_xs. *)
+  (*         rewrite <-NoDup_xs. *)
+  (*         subst m'; clear; revert m. *)
+  (*         induction xs as [|(x', a')]; intros; simpl; try reflexivity. *)
+  (*         rewrite IHxs. *)
+  (*         now rewrite add_inst_val_comm. *)
+  (*       + replace l' with (fst (split ys)); [|now rewrite Eys]. *)
+  (*         intro Hin; apply Notin. *)
+  (*         apply in_split_l' in Hin as (?&?). *)
+  (*         eapply In_InMembers; eauto. *)
+  (*   Qed. *)
+
+  (* End BuildMemWith. *)
+
+  (* Add Parametric Morphism A B V f xs ys m: (fun g => @build_mem_with_spec A B V f g xs ys m) *)
+  (*     with signature (fun g g' => forall x, g x ≋ g' x) ==> equal_memory *)
+  (*       as build_mem_with_spec_rec_equal_memory. *)
+  (* Proof. *)
+  (*   intros g g' E. *)
+  (*   unfold build_mem_with_spec. *)
+  (*   induction ys as [|(y, b)]; simpl; try reflexivity. *)
+  (*   destruct (split ys); simpl. *)
+  (*   unfold Env.adds. simpl. *)
+  (*   destruct (split xs); simpl. *)
+  (*   constructor; try reflexivity. *)
+  (*   simpl. *)
+  (*   inversion_clear IHys as [??? Insts]. *)
+  (*   unfold Env.adds in Insts; simpl in Insts. *)
+  (*   now rewrite E, Insts. *)
+  (* Qed. *)
+
+  (* Fixpoint reset_state_spec (P: SynSB.program) (me: menv) (b: ident) : menv := *)
+  (*   let reset_state_spec_aux (P: SynSB.program) (me: menv) (xb: ident * ident) := *)
+  (*       reset_state_spec P match find_inst (fst xb) me with *)
+  (*                          | Some me' => me' *)
+  (*                          | None => mempty *)
+  (*                          end (snd xb) *)
+  (*   in *)
+  (*   match P with *)
+  (*   | [] => me *)
+  (*   | bl :: P => *)
+  (*     if ident_eqb (b_name bl) b *)
+  (*     then build_mem_with_spec sem_const (reset_state_spec_aux P me) (b_lasts bl) (b_blocks bl) me *)
+  (*     else reset_state_spec P me b *)
+  (*   end. *)
+
+  (* Definition reset_state_spec_aux (P: SynSB.program) (me: menv) (xb: ident * ident) : menv := *)
+  (*   reset_state_spec P match find_inst (fst xb) me with *)
+  (*                      | Some me' => me' *)
+  (*                      | None => mempty *)
+  (*                      end (snd xb). *)
+
+  (* Fixpoint reset_state (P: SynSB.program) (me: menv) (b: ident) : menv := *)
+  (*   let reset_state_aux (P: SynSB.program) (me: menv) (xb: ident * ident) := *)
+  (*       reset_state P match find_inst (fst xb) me with *)
+  (*                          | Some me' => me' *)
+  (*                          | None => mempty *)
+  (*                          end (snd xb) *)
+  (*   in *)
+  (*   match P with *)
+  (*   | [] => me *)
+  (*   | bl :: P => *)
+  (*     if ident_eqb (b_name bl) b *)
+  (*     then build_mem_with sem_const (reset_state_aux P me) (b_lasts bl) (b_blocks bl) me *)
+  (*     else reset_state P me b *)
+  (*   end. *)
+
+  (* Definition reset_state_aux (P: SynSB.program) (me: menv) (xb: ident * ident) : menv := *)
+  (*   reset_state P match find_inst (fst xb) me with *)
+  (*                 | Some me' => me' *)
+  (*                 | None => mempty *)
+  (*                 end (snd xb). *)
+
+  (* Lemma reset_state_equal: *)
+  (*   forall P me b, *)
+  (*     reset_state P me b ≋ reset_state_spec P me b. *)
+  (* Proof. *)
+  (*   induction P as [|bl]; intros; simpl; try reflexivity. *)
+  (*   destruct (ident_eqb (b_name bl) b); auto. *)
+  (*   rewrite (build_mem_with_spec_rec_equal_memory _ _ _ _ _ _ _ _ (reset_state_aux P me)). *)
+  (*   - apply build_mem_with_equal. *)
+  (*     + apply b_nodup_blocks. *)
+  (*     + apply b_nodup_lasts. *)
+  (*   - now setoid_rewrite IHP. *)
+  (* Qed. *)
+
+  (* Lemma reset_state_spec_find_Some: *)
+  (*   forall P me b P' bl, *)
+  (*     find_block b P = Some (bl, P') -> *)
+  (*     reset_state_spec P me b = build_mem_with_spec sem_const *)
+  (*                                                   (reset_state_spec_aux P' me) *)
+  (*                                                   (b_lasts bl) (b_blocks bl) *)
+  (*                                                   me. *)
+  (* Proof. *)
+  (*   intros ** Find. *)
+  (*   induction P as [|bl']. *)
+  (*   - inv Find. *)
+  (*   - simpl in *. *)
+  (*     destruct (ident_eqb (b_name bl') b); auto. *)
+  (*     inv Find; auto. *)
+  (* Qed. *)
+
+  (* Lemma reset_state_spec_find_None: *)
+  (*   forall P me b, *)
+  (*     find_block b P = None -> *)
+  (*     reset_state_spec P me b = me. *)
+  (* Proof. *)
+  (*   intros ** Find. *)
+  (*   induction P as [|bl']; simpl in *; auto. *)
+  (*   destruct (ident_eqb (b_name bl') b); try discriminate; auto. *)
+  (* Qed. *)
+
+  (* Lemma reset_state_find_Some: *)
+  (*   forall P me b P' bl, *)
+  (*     find_block b P = Some (bl, P') -> *)
+  (*     reset_state P me b = build_mem_with sem_const *)
+  (*                                         (reset_state_aux P' me) *)
+  (*                                         (b_lasts bl) (b_blocks bl) *)
+  (*                                         me. *)
+  (* Proof. *)
+  (*   intros ** Find. *)
+  (*   induction P as [|bl']. *)
+  (*   - inv Find. *)
+  (*   - simpl in *. *)
+  (*     destruct (ident_eqb (b_name bl') b); auto. *)
+  (*     inv Find; auto. *)
+  (* Qed. *)
+
+  (* Lemma reset_state_find_None: *)
+  (*   forall P me b, *)
+  (*     find_block b P = None -> *)
+  (*     reset_state P me b = me. *)
+  (* Proof. *)
+  (*   intros ** Find. *)
+  (*   induction P as [|bl']; simpl in *; auto. *)
+  (*   destruct (ident_eqb (b_name bl') b); try discriminate; auto. *)
+  (* Qed. *)
+
+  (* Lemma find_val_reset_state_spec: *)
+  (*   forall P me b bl P', *)
+  (*     find_block b P = Some (bl, P') -> *)
+  (*     (forall x, find_val x me <> None -> InMembers x (b_lasts bl)) -> *)
+  (*     (forall x c, *)
+  (*         In (x, c) (b_lasts bl) -> *)
+  (*         find_val x (reset_state_spec P me b) = Some (sem_const c)) *)
+  (*     /\ *)
+  (*     forall x v, *)
+  (*       find_val x (reset_state_spec P me b) = Some v -> *)
+  (*       exists c, v = sem_const c /\ In (x, c) (b_lasts bl). *)
+  (* Proof. *)
+  (*   intros ** Spec_me. *)
+  (*   unfold find_val in *. *)
+  (*   erewrite reset_state_spec_find_Some; eauto. *)
+  (*   rewrite build_mem_with_spec_values. *)
+  (*   pose proof (b_nodup_lasts_blocks bl) as NoDup. *)
+  (*   apply NoDup_app_weaken in NoDup. *)
+  (*   split; intros ** Hx. *)
+  (*   - destruct (split (b_lasts bl)) eqn: E. *)
+  (*     rewrite <-split_fst_map, E in NoDup; auto. *)
+  (*     apply Env.In_find_adds; auto. *)
+  (*     rewrite combine_map_snd. *)
+  (*     pose proof (split_combine (b_lasts bl)) as Eq. *)
+  (*     rewrite E in Eq. *)
+  (*     apply in_map_iff. *)
+  (*     setoid_rewrite Eq. *)
+  (*     exists (x, c); auto. *)
+  (*   - destruct (Env.find x (values me)) eqn: Find. *)
+  (*     + assert (InMembers x (b_lasts bl)) as Hin *)
+  (*           by (apply Spec_me; rewrite Find; discriminate). *)
+  (*       clear Spec_me. *)
+  (*       induction (b_lasts bl) as [|(x', c')]; simpl in *. *)
+  (*       * inv Hin. *)
+  (*       *{ destruct (split l) eqn: El. *)
+  (*          destruct Hin; simpl in *. *)
+  (*          - subst; rewrite Env.find_gsss in Hx. *)
+  (*            inv Hx; eauto. *)
+  (*          - inversion_clear NoDup as [|?? Notin]. *)
+  (*            rewrite Env.find_gsso in Hx. *)
+  (*            + apply IHl in Hx as (c &?&?); eauto. *)
+  (*            + intro; subst; apply Notin, fst_InMembers; auto. *)
+  (*        } *)
+  (*     + destruct (split (b_lasts bl)) eqn: E. *)
+  (*       rewrite <-split_fst_map, E in NoDup; auto. *)
+  (*       apply Env.find_adds_In in Hx; auto. *)
+  (*       rewrite combine_map_snd in Hx. *)
+  (*       pose proof (split_combine (b_lasts bl)) as Eq. *)
+  (*       rewrite E in Eq. *)
+  (*       apply in_map_iff in Hx as ((?&?)& E' & Hin). *)
+  (*       inv E'; setoid_rewrite Eq in Hin. *)
+  (*       exists c; auto. *)
+  (* Qed. *)
+
+  (* Lemma reset_state_spec_other: *)
+  (*   forall P P' b me bl, *)
+  (*     find_block b P = None -> *)
+  (*     b <> b_name bl -> *)
+  (*     reset_state_spec (P ++ bl :: P') me b = reset_state_spec P' me b. *)
+  (* Proof. *)
+  (*   intros. *)
+  (*   destruct (find_block b P') as [[]|] eqn: Find. *)
+  (*   - symmetry; erewrite reset_state_spec_find_Some; eauto. *)
+  (*     erewrite <-find_block_other_app in Find; eauto. *)
+  (*     erewrite reset_state_spec_find_Some; eauto. *)
+  (*   - symmetry; rewrite reset_state_spec_find_None; auto. *)
+  (*     rewrite <-find_block_other_app with (P := P) (bl := bl) in Find; eauto. *)
+  (*     rewrite reset_state_spec_find_None; auto. *)
+  (* Qed. *)
+
+  (* Lemma initial_reset_state_spec: *)
+  (*   forall P me b P' bl, *)
+  (*     Ordered_blocks P -> *)
+  (*     find_block b P = Some (bl, P') -> *)
+  (*     (forall x, find_val x me <> None -> InMembers x (b_lasts bl)) -> *)
+  (*     initial_state P b (reset_state_spec P me b). *)
+  (* Proof. *)
+  (*   induction P; try now inversion 1. *)
+  (*   intros ** Ord Find Spec_me. *)
+  (*   econstructor; eauto. *)
+  (*   - split; eapply find_val_reset_state_spec; eauto. *)
+  (*   - intros. *)
+  (*     unfold sub_inst, find_inst. *)
+  (*     erewrite reset_state_spec_find_Some; eauto. *)
+  (*     rewrite build_mem_with_spec_instances. *)
+  (*     pose proof (b_nodup_lasts_blocks bl) as NoDup. *)
+  (*     apply NoDup_comm, NoDup_app_weaken in NoDup. *)
+  (*     destruct (split (b_blocks bl)) as (l, l') eqn: Eq. *)
+  (*     simpl. *)
+  (*     exists (reset_state_spec P' b'); split. *)
+  (*     + apply Environment.Env.In_find_adds. *)
+  (*       * assert (l = map fst (b_blocks bl)) as -> by (now rewrite <-split_fst_map, Eq); auto. *)
+  (*       * rewrite combine_map_snd. *)
+  (*         apply in_map_iff. *)
+  (*         exists (x, b'); split; auto. *)
+  (*         pose proof (split_combine (b_blocks bl)) as Eq'. *)
+  (*         rewrite Eq in Eq';  setoid_rewrite Eq'; auto. *)
+  (*     + simpl in Find. *)
+  (*       destruct (ident_eqb (b_name a) b) eqn: E. *)
+  (*       * inv Find. *)
+  (*         pose proof Ord as Ord'. *)
+  (*         inversion_clear Ord as [|??? Blocks]. *)
+  (*         eapply Forall_forall in Blocks as (?&?&?&Find'); eauto. *)
+  (*         apply IHP in Find'; auto. *)
+  (*         rewrite <-initial_state_tail; auto. *)
+  (*       * pose proof Ord as Ord'. *)
+  (*         inversion_clear Ord as [|?? Ord'' Blocks]; clear Blocks. *)
+  (*         apply find_block_app in Find as (P1 & HP &?). *)
+  (*         rewrite HP in *. *)
+  (*         apply Ordered_blocks_split in Ord''. *)
+  (*         eapply Forall_forall in Ord'' as (?&?&?&?& Find'); eauto. *)
+  (*         simpl in *. *)
+  (*         rewrite <-find_block_other_app with (P := P1) (bl := bl) in Find'; auto. *)
+  (*         pose proof Ord'. *)
+  (*         inversion_clear Ord'. *)
+  (*         pose proof Find' as Find. *)
+  (*         apply IHP in Find'; auto. *)
+  (*         rewrite reset_state_spec_other in Find'; auto. *)
+  (*         rewrite <-initial_state_tail; auto. *)
+  (*         pose proof Find as Find_name; apply find_block_name in Find_name. *)
+  (*         rewrite <-Find_name. *)
+  (*         apply find_block_In in Find. *)
+  (*         eapply Forall_forall in Find; eauto. *)
+  (*         apply Find. *)
+  (* Qed. *)
+
+  (* Corollary initial_reset_state: *)
+  (*   forall P b P' bl, *)
+  (*     Ordered_blocks P -> *)
+  (*     find_block b P = Some (bl, P') -> *)
+  (*     initial_state P b (reset_state P b). *)
+  (* Proof. *)
+  (*   intros. *)
+  (*   rewrite reset_state_equal. *)
+  (*   eapply initial_reset_state_spec; eauto. *)
+  (* Qed. *)
+
+  Lemma stmt_call_eval_cons:
+    forall prog c' c me f vs me' rvs,
+      c_name c <> c' ->
+      (stmt_call_eval (c :: prog) me c' f vs me' rvs
+       <-> stmt_call_eval prog me c' f vs me' rvs).
   Proof.
-    induction P as [|bl]; intros; simpl; try reflexivity.
-    destruct (ident_eqb (b_name bl) b); auto.
-    rewrite (build_mem_with_spec_rec_equal_memory _ _ _ _ _ _ _ _ (reset_state P)).
-    - apply build_mem_with_equal.
-      + apply b_nodup_blocks.
-      + apply b_nodup_lasts.
-    - now setoid_rewrite IHP.
+    intros ** Neq; rewrite <-ident_eqb_neq in Neq; split; intros Sem.
+    - inversion_clear Sem as [??????????? Find].
+      simpl in Find; rewrite Neq in Find; eauto using stmt_call_eval.
+    - inv Sem; econstructor; eauto.
+      simpl; rewrite Neq; auto.
   Qed.
 
-  Lemma reset_state_spec_find_Some:
-    forall P b P' bl,
-      find_block b P = Some (bl, P') ->
-      reset_state_spec P b = build_mem_with_spec sem_const
-                                                 (reset_state_spec P')
-                                                 (b_lasts bl) (b_blocks bl)
-                                                 (empty_memory _).
-  Proof.
-    intros ** Find.
-    induction P as [|bl'].
-    - inv Find.
-    - simpl in *.
-      destruct (ident_eqb (b_name bl') b); auto.
-      inv Find; auto.
-  Qed.
+  (* Lemma fuu: *)
+  (*   forall P b P' bl me, *)
+  (*     Ordered_blocks P -> *)
+  (*     find_block b P = Some (bl, P') -> *)
+  (*     stmt_call_eval (translate P) me b reset [] (reset_state P me b) []. *)
+  (* Proof. *)
+  (*   induction P as [|bl']; try now inversion 2. *)
+  (*   intros ** Ord Find. *)
+  (*   pose proof Find as Find'. *)
+  (*   simpl in Find. *)
+  (*   destruct (ident_eqb (b_name bl') b) eqn: E. *)
+  (*   - inv Find. *)
+  (*     (* pose proof Ord as Ord'. *) *)
+  (*     (* inversion_clear Ord' as [|??? Blocks]; clear Blocks. *) *)
+  (*     (* pose proof Find as Find'. *) *)
+  (*     (* apply find_block_app in Find' as (P1 & Hp &?); rewrite Hp in *. *) *)
+  (*     (* apply Ordered_blocks_split in Ord. *) *)
+  (*     erewrite reset_state_find_Some; eauto. *)
+  (*     pose proof Find' as Find_c; apply find_block_translate in Find_c as (?&?&?&?&?); subst. *)
+  (*     econstructor; eauto. *)
+  (*     + apply exists_reset_method. *)
+  (*     + instantiate (1 := vempty). *)
+  (*       simpl; rewrite Env.adds_nil_nil. *)
+  (*       unfold translate_reset_eqns, build_mem_with. *)
+  (*       inversion_clear Ord as [|??? Blocks]. *)
+  (*       revert me. *)
+  (*       induction (b_blocks bl) as [|(inst, b')]; simpl. *)
+  (*       * induction (b_lasts bl) as [|(x, c)]; simpl; intro; eauto using stmt_eval. *)
+  (*         rewrite stmt_eval_fold_left_lift. *)
+  (*         do 2 eexists; split; eauto using stmt_eval, exp_eval. *)
+  (*       *{ induction (b_lasts bl) as [|(x, c)]; simpl in *; intro; eauto using stmt_eval. *)
+  (*          - rewrite stmt_eval_fold_left_lift. *)
+  (*            inversion Blocks as [|?? (?&?&?&?) Blocks']; subst; simpl in *; *)
+  (*              eauto. *)
+  (*            do 2 eexists; split; eauto using stmt_eval. *)
+  (*            unfold reset_state_aux at 2; simpl. *)
+  (*            set (me' := add_inst inst (reset_state P' match find_inst inst me with *)
+  (*                                   | Some om => om *)
+  (*                                   | None => mempty *)
+  (*                                   end b') me). *)
+  (*            apply IHl.  *)
+  (*            rewrite Env.adds_nil_nil. *)
+  (*            apply IHl with (me := add_inst inst (reset_state_aux P' me (inst, b')) me) in Blocks'. *)
+  (*            unfold reset_state_aux in *; simpl in *. *)
+  (*            apply Blocks'.  *)
 
-  Lemma reset_state_spec_find_None:
-    forall P b,
-      find_block b P = None ->
-      reset_state_spec P b = empty_memory _.
-  Proof.
-    intros ** Find.
-    induction P as [|bl']; simpl in *; auto.
-    destruct (ident_eqb (b_name bl') b); try discriminate; auto.
-  Qed.
+  (*              apply IHl.  *)
+  (*              eapply IHP; eauto.  *)
 
-  Lemma reset_state_find_Some:
-    forall P b P' bl,
-      find_block b P = Some (bl, P') ->
-      reset_state P b = build_mem_with sem_const
-                                       (reset_state P')
-                                       (b_lasts bl) (b_blocks bl)
-                                       (empty_memory _).
-  Proof.
-    intros ** Find.
-    induction P as [|bl'].
-    - inv Find.
-    - simpl in *.
-      destruct (ident_eqb (b_name bl') b); auto.
-      inv Find; auto.
-  Qed.
+  (*              rewrite find_inst_gempty. *)
+  (*            inversion Blocks as [|?? (?&?&?& Find)]; subst; simpl in *. *)
+  (*            pose proof Find as Find_c.  *)
+  (*            rewrite stmt_call_eval_cons; auto.  *)
+  (*            (* rewrite <-find_block_other_app with (P:=P1) (bl:=bl) in Find'; auto. *) *)
+  (*            (* pose proof Find' as Find_c. *) *)
+  (*            apply find_block_translate in Find_c as (?&?&?&?&?); subst. *)
+  (*            econstructor; eauto. *)
+  (*            + apply exists_reset_method. *)
+  (*            + simpl; rewrite Env.adds_nil_nil. *)
 
-  Lemma reset_state_find_None:
-    forall P b,
-      find_block b P = None ->
-      reset_state P b = empty_memory _.
-  Proof.
-    intros ** Find.
-    induction P as [|bl']; simpl in *; auto.
-    destruct (ident_eqb (b_name bl') b); try discriminate; auto.
-  Qed.
+  (*            SearchAbout find_class find_block. apply find_block_translate. *)
+  (*         SearchAbout empty_memory. *)
+  (*     econstructor; eauto using exp_eval. *)
 
-  Lemma find_val_reset_state_spec:
-    forall P b bl P',
-      find_block b P = Some (bl, P') ->
-      (forall x c,
-          In (x, c) (b_lasts bl) ->
-          find_val x (reset_state_spec P b) = Some (sem_const c))
-      /\
-      forall x v,
-        find_val x (reset_state_spec P b) = Some v ->
-        exists c, v = sem_const c /\ In (x, c) (b_lasts bl).
-  Proof.
-    intros.
-    unfold find_val.
-    erewrite reset_state_spec_find_Some; eauto.
-    rewrite build_mem_with_spec_values.
-    pose proof (b_nodup_lasts_blocks bl) as NoDup.
-    apply NoDup_app_weaken in NoDup.
-    induction (b_lasts bl) as [|(x', c')]; simpl.
-    - rewrite Env.adds_nil_nil; setoid_rewrite Env.gempty.
-      split; [contradiction | discriminate].
-    - destruct (split l); simpl.
-      inversion_clear NoDup as [|?? Notin].
-      split; [intros ** [Eq|?]|intros ** Find].
-      + inv Eq; apply Env.find_gsss.
-      + rewrite Env.find_gsso; auto.
-        * now apply IHl.
-        * intro; subst; apply Notin.
-          apply in_map_iff; exists (x', c); auto.
-      + destruct (ident_eq_dec x x').
-        * subst; rewrite Env.find_gsss in Find; inv Find; eauto.
-        * rewrite Env.find_gsso in Find; auto.
-          apply IHl in Find as (?&?&?); eauto.
-  Qed.
+  (* Lemma fuu: *)
+  (*   forall P b P' bl, *)
+  (*     Ordered_blocks P -> *)
+  (*     find_block b P = Some (bl, P') -> *)
+  (*     stmt_eval (translate P) mempty vempty (translate_reset_eqns bl) (reset_state P b, vempty). *)
+  (* Proof. *)
+  (*   induction P as [|bl']; try now inversion 2. *)
+  (*   intros ** Ord Find. *)
+  (*   pose proof Find as Find'. *)
+  (*   simpl in Find. *)
+  (*   destruct (ident_eqb (b_name bl') b) eqn: E. *)
+  (*   - inv Find. *)
+  (*     (* pose proof Ord as Ord'. *) *)
+  (*     (* inversion_clear Ord' as [|??? Blocks]; clear Blocks. *) *)
+  (*     (* pose proof Find as Find'. *) *)
+  (*     (* apply find_block_app in Find' as (P1 & Hp &?); rewrite Hp in *. *) *)
+  (*     (* apply Ordered_blocks_split in Ord. *) *)
+  (*     erewrite reset_state_find_Some; eauto. *)
+  (*     unfold translate_reset_eqns, build_mem_with. *)
+  (*     inversion_clear Ord as [|??? Blocks]. *)
+  (*     induction (b_blocks bl) as [|(inst, b')]; simpl. *)
+  (*     + generalize mempty. *)
+  (*       induction (b_lasts bl) as [|(x, c)]; simpl; eauto using stmt_eval. *)
+  (*       intro. *)
+  (*       rewrite stmt_eval_fold_left_lift. *)
+  (*       do 2 eexists; split; eauto using stmt_eval, exp_eval. *)
+  (*     + induction (b_lasts bl) as [|(x, c)]; simpl in *; eauto using stmt_eval. *)
+  (*       *{ rewrite stmt_eval_fold_left_lift. *)
+  (*          do 2 eexists; split. *)
+  (*          - econstructor; eauto using stmt_eval. *)
+  (*            econstructor; eauto. *)
+  (*            rewrite find_inst_gempty. *)
+  (*            inversion Blocks as [|?? (?&?&?& Find)]; subst; simpl in *. *)
+  (*            pose proof Find as Find_c.  *)
+  (*            rewrite stmt_call_eval_cons; auto.  *)
+  (*            (* rewrite <-find_block_other_app with (P:=P1) (bl:=bl) in Find'; auto. *) *)
+  (*            (* pose proof Find' as Find_c. *) *)
+  (*            apply find_block_translate in Find_c as (?&?&?&?&?); subst. *)
+  (*            econstructor; eauto. *)
+  (*            + apply exists_reset_method. *)
+  (*            + simpl; rewrite Env.adds_nil_nil. *)
 
-  Lemma reset_state_spec_other:
-    forall P P' b bl,
-      find_block b P = None ->
-      b <> b_name bl ->
-      reset_state_spec (P ++ bl :: P') b = reset_state_spec P' b.
-  Proof.
-    intros.
-    destruct (find_block b P') as [[]|] eqn: Find.
-    - symmetry; erewrite reset_state_spec_find_Some; eauto.
-      erewrite <-find_block_other_app in Find; eauto.
-      erewrite reset_state_spec_find_Some; eauto.
-    - symmetry; rewrite reset_state_spec_find_None; auto.
-      rewrite <-find_block_other_app with (P := P) (bl := bl) in Find; eauto.
-      rewrite reset_state_spec_find_None; auto.
-  Qed.
-
-  Lemma initial_reset_state_spec:
-    forall P b P' bl,
-      Ordered_blocks P ->
-      find_block b P = Some (bl, P') ->
-      initial_state P b (reset_state_spec P b).
-  Proof.
-    induction P; try now inversion 1.
-    intros ** Ord Find.
-    econstructor; eauto.
-    - split; eapply find_val_reset_state_spec; eauto.
-    - intros.
-      unfold sub_inst, find_inst.
-      erewrite reset_state_spec_find_Some; eauto.
-      rewrite build_mem_with_spec_instances.
-      pose proof (b_nodup_lasts_blocks bl) as NoDup.
-      apply NoDup_comm, NoDup_app_weaken in NoDup.
-      destruct (split (b_blocks bl)) as (l, l') eqn: Eq.
-      simpl.
-      exists (reset_state_spec P' b'); split.
-      + apply Environment.Env.In_find_adds.
-        * assert (l = map fst (b_blocks bl)) as -> by (now rewrite <-split_fst_map, Eq); auto.
-        * rewrite combine_map_snd.
-          apply in_map_iff.
-          exists (x, b'); split; auto.
-          pose proof (split_combine (b_blocks bl)) as Eq'.
-          rewrite Eq in Eq';  setoid_rewrite Eq'; auto.
-      + simpl in Find.
-        destruct (ident_eqb (b_name a) b) eqn: E.
-        * inv Find.
-          pose proof Ord as Ord'.
-          inversion_clear Ord as [|??? Blocks].
-          eapply Forall_forall in Blocks as (?&?&?&Find'); eauto.
-          apply IHP in Find'; auto.
-          rewrite <-initial_state_tail; auto.
-        * pose proof Ord as Ord'.
-          inversion_clear Ord as [|?? Ord'' Blocks]; clear Blocks.
-          apply find_block_app in Find as (P1 & HP &?).
-          rewrite HP in *.
-          apply Ordered_blocks_split in Ord''.
-          eapply Forall_forall in Ord'' as (?&?&?&?& Find'); eauto.
-          simpl in *.
-          rewrite <-find_block_other_app with (P := P1) (bl := bl) in Find'; auto.
-          pose proof Ord'.
-          inversion_clear Ord'.
-          pose proof Find' as Find.
-          apply IHP in Find'; auto.
-          rewrite reset_state_spec_other in Find'; auto.
-          rewrite <-initial_state_tail; auto.
-          pose proof Find as Find_name; apply find_block_name in Find_name.
-          rewrite <-Find_name.
-          apply find_block_In in Find.
-          eapply Forall_forall in Find; eauto.
-          apply Find.
-  Qed.
-
-  Corollary initial_reset_state:
-    forall P b P' bl,
-      Ordered_blocks P ->
-      find_block b P = Some (bl, P') ->
-      initial_state P b (reset_state P b).
-  Proof.
-    intros.
-    rewrite reset_state_equal.
-    eapply initial_reset_state_spec; eauto.
-  Qed.
+  (*            SearchAbout find_class find_block. apply find_block_translate. *)
+  (*         SearchAbout empty_memory. *)
+  (*     econstructor; eauto using exp_eval. *)
 
 
-  (* SearchAbout Comp.  *)
-  Lemma fuu:
-    forall P b P' prog bl,
-      find_block b P = Some (bl, P') ->
-      stmt_eval prog (empty_memory _) vempty (translate_reset_eqns bl) (reset_state P b, vempty).
-  Proof.
-    induction P; try now inversion 1.
-    intros.
-    erewrite reset_state_find_Some; eauto.
-    unfold translate_reset_eqns, build_mem_with.
-    rewrite stmt_eval_fold_left_shift.
-    induction (b_blocks bl) as [|(inst, b')]; simpl.
-    - induction (b_lasts bl) as [|(x, c)]; simpl; eauto using stmt_eval.
-
-      destruct l; simpl.
-      + econstructor.
-    -
+  (*     destruct l; simpl. *)
+  (*     + econstructor. *)
+  (*   - *)
 
 
-    reset_state. reset_method; simpl.
+  (*   reset_state. reset_method; simpl. *)
 
 
 
-  Lemma call_reset:
-    forall P b me bl P',
-      find_block b P = Some (bl, P') ->
-      exists me',
-        stmt_call_eval (translate P) me b reset [] me' []
-        /\ initial_state P b me'.
-  Proof.
-    intros ** Find.
-    apply find_block_translate in Find as (?&?&?&?).
-    eexists; split.
-    - econstructor; eauto.
-      + subst; apply exists_reset_method.
-      + rewrite Env.adds_nil_nil. SearchAbout Env.adds nil. SearchAbout find_method reset.
-  Admitted.
+  (* Lemma call_reset: *)
+  (*   forall P b me bl P', *)
+  (*     find_block b P = Some (bl, P') -> *)
+  (*     exists me', *)
+  (*       stmt_call_eval (translate P) me b reset [] me' [] *)
+  (*       /\ initial_state P b me'. *)
+  (* Proof. *)
+  (*   intros ** Find. *)
+  (*   apply find_block_translate in Find as (?&?&?&?). *)
+  (*   eexists; split. *)
+  (*   - econstructor; eauto. *)
+  (*     + subst; apply exists_reset_method. *)
+  (*     + rewrite Env.adds_nil_nil. SearchAbout Env.adds nil. SearchAbout find_method reset. *)
+  (* Admitted. *)
 
-  Section BaseTrue.
+  Ltac cases :=
+    repeat match goal with
+           | H: context [ match negb ?x with _ => _ end ] |- _ => destruct x; simpl; try solve [inv H; auto]
+           | H: context [ match ?x with _ => _ end ] |- _ => destruct x; try solve [inv H; auto]
+           | |- context [ match negb ?x with _ => _ end ] => destruct x; simpl
+           | |- context [ match ?x with _ => _ end ] => destruct x
+           end; auto.
 
-    Variable (R: env) (mems: PS.t).
-    Variable (me: menv) (ve: venv).
+  Section Expr.
+
+    Variable (mems: PS.t).
 
     Lemma typeof_correct:
-      forall e, typeof (translate_lexp mems e) = ExprSyn.typeof e.
+      forall e,
+        typeof (translate_lexp mems e) = ExprSyn.typeof e.
     Proof.
-      induction e; simpl; auto.
-      destruct (PS.mem i mems); auto.
+      induction e; intros; simpl; auto; cases.
     Qed.
 
-    Hypothesis Compat_env: compat_env R mems me ve.
+    Variable (R: env).
+    Variable (me: menv) (ve: venv).
 
     Lemma lexp_correct:
       forall e c,
         sem_lexp_instant true R e (present c) ->
+        equiv_env (fun x => Is_free_in_lexp x e) R mems me ve ->
         exp_eval me ve (translate_lexp mems e) c.
     Proof.
       induction e;
-        inversion_clear 1 as [|??? Hvar| | | | | | |]; simpl; auto.
+        inversion_clear 1 as [|??? Hvar| | | | | | |];
+        simpl; intros ** Equiv; auto.
       - constructor; congruence.
-      - apply Compat_env in Hvar.
-        destruct (PS.mem i mems); eauto using exp_eval.
+      - apply Equiv in Hvar; auto using Is_free_in_lexp.
+        cases; eauto using exp_eval.
       - econstructor; eauto.
         now rewrite typeof_correct.
       - econstructor; eauto.
@@ -406,106 +779,236 @@ Module Type CORRECTNESS
     Corollary lexps_correct:
       forall es cs,
         sem_lexps_instant true R es (map present cs) ->
+        equiv_env (fun x => Exists (Is_free_in_lexp x) es) R mems me ve ->
         Forall2 (exp_eval me ve) (map (translate_lexp mems) es) cs.
     Proof.
       setoid_rewrite Forall2_map_1; setoid_rewrite Forall2_map_2;
-        intros; eapply Forall2_impl_In; eauto; auto.
+        intros; eapply Forall2_impl_In; eauto.
+      intros; apply lexp_correct; auto.
+      weaken_equiv_env with (setoid_rewrite Exists_exists; eauto).
     Qed.
     Hint Resolve lexps_correct.
 
     Lemma cexp_correct:
       forall e c prog x,
         sem_cexp_instant true R e (present c) ->
+        equiv_env (fun x => Is_free_in_cexp x e) R mems me ve ->
         stmt_eval prog me ve (translate_cexp mems x e) (me, Env.add x c ve).
     Proof.
       induction e;
         inversion 1 as [???? Hvar|???? Hvar| | | |];
-        subst; simpl; eauto.
-      - apply Compat_env in Hvar.
+        subst; simpl; intros ** Equiv; eauto using stmt_eval.
+      - apply Equiv in Hvar; auto using Is_free_in_cexp.
         econstructor; eauto.
         + unfold bool_var, tovar.
-          destruct (PS.mem i mems); eauto using exp_eval.
+          cases; eauto using exp_eval.
         + apply val_to_bool_true.
         + simpl; auto.
-      - apply Compat_env in Hvar.
+      - apply Equiv in Hvar; auto using Is_free_in_cexp.
         econstructor; eauto.
         + unfold bool_var, tovar.
-          destruct (PS.mem i mems); eauto using exp_eval.
+          cases; eauto using exp_eval.
         + apply val_to_bool_false.
         + simpl; auto.
       - econstructor; eauto.
-        destruct b; match goal with H: present _ = present _ |- _ => inv H end; auto.
+        cases.
     Qed.
     Hint Resolve cexp_correct.
 
-    Lemma stmt_eval_Control:
-      forall ck prog s,
-        (sem_clock_instant true R ck false ->
-         stmt_eval prog me ve (Control mems ck s) (me, ve))
-        /\
-        (forall me' ve',
-            sem_clock_instant true R ck true ->
-            stmt_eval prog me ve s (me', ve') ->
-            stmt_eval prog me ve (Control mems ck s) (me', ve')).
-    Proof.
-      induction ck; split;
-        inversion_clear 1 as [ |????? Hvar| |????? Hvar]; simpl; auto.
-      - destruct b; edestruct IHck; eauto.
-      - apply Compat_env in Hvar.
-        unfold bool_var, tovar.
-        destruct b0; simpl;
-          destruct (PS.mem i mems); eapply IHck; eauto using stmt_eval, exp_eval.
-      - apply Compat_env in Hvar.
-        unfold bool_var, tovar.
-        intros; destruct b;
-          destruct (PS.mem i mems); eapply IHck; eauto using stmt_eval, exp_eval.
-    Qed.
+    Section Clock.
 
-    Corollary stmt_eval_Control_absent:
-      forall ck prog s,
-        sem_clock_instant true R ck false ->
-        stmt_eval prog me ve (Control mems ck s) (me, ve).
-    Proof. apply stmt_eval_Control. Qed.
+      Variable ck: clock.
+      Hypothesis Equiv: equiv_env (fun x => Is_free_in_clock x ck) R mems me ve.
 
-    Corollary stmt_eval_Control_present:
-      forall ck prog s me' ve',
-        sem_clock_instant true R ck true ->
-        stmt_eval prog me ve s (me', ve') ->
-        stmt_eval prog me ve (Control mems ck s) (me', ve').
-    Proof. apply stmt_eval_Control. Qed.
+      Lemma stmt_eval_Control:
+        forall prog s,
+          (sem_clock_instant true R ck false ->
+           stmt_eval prog me ve (Control mems ck s) (me, ve))
+          /\
+          (forall me' ve',
+              sem_clock_instant true R ck true ->
+              stmt_eval prog me ve s (me', ve') ->
+              stmt_eval prog me ve (Control mems ck s) (me', ve')).
+      Proof.
+        induction ck; split;
+          inversion_clear 1 as [ |????? Hvar| |????? Hvar];
+          simpl; intros; auto.
+        - cases; edestruct IHc; eauto.
+        - apply Equiv in Hvar; auto using Is_free_in_clock.
+          unfold bool_var, tovar.
+          cases; eapply IHc; eauto using stmt_eval, exp_eval.
+        - apply Equiv in Hvar; auto using Is_free_in_clock.
+          unfold bool_var, tovar.
+          cases; eapply IHc; eauto using stmt_eval, exp_eval.
+      Qed.
 
-    Lemma foo:
-      forall P S I S' eq,
-        sem_equation P true R S I S' eq ->
-        exists me' ve',
-          stmt_eval (translate P) me ve (translate_eqn mems eq) (me', ve').
-    Proof.
-      destruct eq;
-        inversion_clear 1 as [????????? Hexp|
-                              ???????????? Hexp|
-                              ????????????? Init|
-                              ???????????????? Hexps]; simpl.
-      - inv Hexp;
-          eauto using stmt_eval_Control_absent, stmt_eval_Control_present, cexp_correct.
-      - inv Hexp;
-          eauto 6 using stmt_eval_Control_absent, stmt_eval_Control_present, stmt_eval.
-      - destruct r; eauto using stmt_eval_Control_absent.
-        inversion_clear Init as [???? Find Rst].
-        apply find_block_translate in Find as (?&?&?&?).
+      Corollary stmt_eval_Control_absent:
+        forall prog s,
+          sem_clock_instant true R ck false ->
+          stmt_eval prog me ve (Control mems ck s) (me, ve).
+      Proof. apply stmt_eval_Control. Qed.
+
+      Corollary stmt_eval_Control_present:
+        forall prog s me' ve',
+          sem_clock_instant true R ck true ->
+          stmt_eval prog me ve s (me', ve') ->
+          stmt_eval prog me ve (Control mems ck s) (me', ve').
+      Proof. apply stmt_eval_Control. Qed.
+
+    End Clock.
+
+  End Expr.
+
+  (* Lemma fuu: *)
+  (*   forall eqs R x c prog me ve me' ve' mems, *)
+  (*     sem_var_instant R x (present c) -> *)
+  (*     Is_variable_in_eqs x eqs -> *)
+  (*     stmt_eval prog me ve (translate_eqns mems eqs) (me', ve') -> *)
+  (*     Env.find x ve' = Some c. *)
+  (* Proof. *)
+  (*   unfold translate_eqns. *)
+  (*   induction eqs as [|[]]; *)
+  (*     inversion_clear 2 as [?? Hlol|]; try inv Hlol; simpl; intros ** StEval. *)
+  (*   - apply stmt_eval_fold_left_shift in StEval as (?&?&?& StEval). *)
+  (*     inversion_clear StEval as [| | |????????? StEval' EvalSkip| |]; inv EvalSkip. *)
+
+  (*     inv StEval'. *)
+  (*   inv H0. *)
+
+  Lemma equation_cons_correct:
+    forall eq eqs P R S I S' me ve inputs mems,
+      sem_equation P true R S I S' eq ->
+      Is_well_sch inputs mems (eq :: eqs) ->
+      Memory_Corres_eqs P S' me eqs ->
+      Memory_Corres_eq P S me eq ->
+      equiv_env (fun x => Is_free_in_eq x eq) R mems me ve ->
+      exists me' ve',
+        stmt_eval (translate P) me ve (translate_eqn mems eq) (me', ve')
+        /\ Memory_Corres_eqs P S' me' (eq :: eqs).
+  Proof.
+    inversion_clear 1 as [????????? Hexp|
+                          ???????????? Hexp|
+                          ???????????? Init|
+                          ??????????????? Hexps];
+      inversion_clear 1;
+      inversion_clear 2;
+      intros; simpl.
+
+    - inv Hexp; exists me; eexists; split;
+        try solve [eapply stmt_eval_Control_absent; eauto; auto];
+        try constructor; auto using Memory_Corres_eq; eauto; auto.
+      eapply stmt_eval_Control_present; eauto; auto.
+      eapply cexp_correct; eauto.
+
+    - inv Hexp; eexists; exists ve; split;
+        try solve [eapply stmt_eval_Control_absent; eauto; auto].
+      + eapply stmt_eval_Control_present; eauto using stmt_eval, lexp_correct; auto.
+      + constructor; auto.
+        * constructor.
+          setoid_rewrite find_val_gss; congruence.
+        * apply Memory_Corres_eqs_add_val; auto.
+      + do 2 (constructor; auto); intros.
+        match goal with
+        | H: find_val ?x ?S' = _, H': find_val ?x ?S' = _ |- _ =>
+          rewrite H in H'; inv H'; auto
+        end.
+
+    - destruct r.
+      + inversion_clear Init as [???? Find Rst].
+        apply find_block_translate in Find as (?&?&?&?&?); subst.
         admit.
-        (* do 2 eexists. *)
-        (* apply stmt_eval_Control_present; auto. *)
-        (* econstructor; eauto. *)
-
-        (* econstructor; eauto. *)
-        (* + subst; apply exists_reset_method. *)
-      - inv Hexps; eauto using stmt_eval_Control_absent.
+      + exists me, ve; split; try eapply stmt_eval_Control_absent; eauto; auto.
+        constructor; auto.
+        constructor.
         admit.
-        (* do 2 eexists. *)
-        (* apply stmt_eval_Control_present; auto. *)
-        (* econstructor; eauto. *)
-    Qed.
 
-  End BaseTrue.
+    - inv Hexps.
+      + admit.
+      + exists me, ve; split; try eapply stmt_eval_Control_absent; eauto; auto.
+        constructor; auto.
+        constructor.
+        intros.
+        match goal with
+        | H: sub_inst ?s ?S' _, H': sub_inst ?s ?S' _ |- _ =>
+          unfold sub_inst in H, H'; rewrite H in H'; inv H'; auto
+        end.
+        admit.
+
+  Qed.
+
+  Lemma foo:
+    forall P S me ve me' ve' eqs eq mems,
+      Memory_Corres_eq P S me eq ->
+      stmt_eval (translate P) me ve (translate_eqns mems eqs) (me', ve') ->
+      Memory_Corres_eq P S me' eq.
+  Proof.
+    induction 1.
+    intros.
+
+    destruct eq.
+
+  Admitted.
+
+
+  Lemma equations_cons_correct:
+    forall eq eqs P R S I S' me ve me' ve' inputs mems,
+      sem_equation P true R S I S' eq ->
+      Is_well_sch inputs mems (eq :: eqs) ->
+      Memory_Corres_eqs P S' me' eqs ->
+      Memory_Corres_eq P S me eq ->
+      equiv_env (fun x => Is_free_in_eq x eq) R mems me' ve' ->
+      stmt_eval (translate P) me ve (translate_eqns mems eqs) (me', ve') ->
+      exists me'' ve'',
+        stmt_eval (translate P) me ve (translate_eqns mems (eq :: eqs)) (me'', ve'')
+        /\ Memory_Corres_eqs P S' me'' (eq :: eqs).
+  Proof.
+    intros.
+    edestruct equation_cons_correct as (me'' & ve'' &?&?); eauto.
+    exists me'', ve''; split; auto.
+    unfold translate_eqns; simpl; rewrite stmt_eval_fold_left_shift.
+    exists me', ve'; split; eauto using stmt_eval.
+  Qed.
+
+  Lemma equations_correct:
+    forall eqs P R S I S' me ve inputs mems,
+      Forall (sem_equation P true R S I S') eqs ->
+      Is_well_sch inputs mems eqs ->
+      Memory_Corres_eqs P S me eqs ->
+      exists me' ve',
+        stmt_eval (translate P) me ve (translate_eqns mems eqs) (me', ve')
+        /\ Memory_Corres_eqs P S' me' eqs.
+  Proof.
+    induction eqs; simpl;
+      intros ** Heqs Wsch Corres; inv Heqs; inv Wsch; inv Corres.
+    - do 4 econstructor.
+    - edestruct IHeqs as (me' & ve' &?&?); eauto.
+      eapply equations_cons_correct; eauto using Is_well_sch.
+      admit.
+  Qed.
+
+  Theorem correctness:
+    forall P b S xs ys S' me,
+      sem_block P b S (map present xs) (map present ys) S' ->
+      Memory_Corres P b S me ->
+      exists me',
+        stmt_call_eval (translate P) me b step xs me' ys
+        /\ Memory_Corres P b S' me'.
+  Proof.
+    intros ** Sem Corres.
+    inversion_clear Sem as [?????????? Clock Find ????? Heqs IHeqs].
+    inversion_clear Corres as [????? Find']; rewrite Find' in Find; inv Find.
+    assert (Is_well_sch (map fst (b_in bl)) (ps_from_list (map fst (b_lasts bl))) (b_eqs bl)) by admit.
+    assert (base = true) by (apply Clock; rewrite present_list_spec; eauto); subst.
+    edestruct equations_correct with (ve := Env.adds (map fst (m_in (step_method bl))) xs vempty)
+      as (me' & ve' &?&?); eauto.
+    exists me'; split; eauto using Memory_Corres.
+    apply find_block_translate in Find' as (?&?&?&?&?); subst.
+    econstructor; eauto.
+    - apply exists_step_method.
+    - instantiate (1 := ve').
+      admit.
+    - admit.
+  Qed.
+
 
 End CORRECTNESS.
